Compiler/CompilationModel/LogicalPurity.lean
@@ -34,7 +34,8 @@ partial def exprContainsCallLike (expr : Expr) : Bool :=
   | Expr.sar a b | Expr.signextend a b |
     Expr.eq a b | Expr.ge a b | Expr.gt a b | Expr.sgt a b | Expr.lt a b | Expr.slt a b | Expr.le a b |
     Expr.logicalAnd a b | Expr.logicalOr a b |
-    Expr.wMulDown a b | Expr.wDivUp a b | Expr.min a b | Expr.max a b =>
+    Expr.wMulDown a b | Expr.wDivUp a b | Expr.min a b | Expr.max a b |
+    Expr.ceilDiv a b =>
       exprContainsCallLike a || exprContainsCallLike b
   | Expr.mulDivDown a b c | Expr.mulDivUp a b c =>
       exprContainsCallLike a || exprContainsCallLike b || exprContainsCallLike c
@@ -115,7 +116,7 @@ def exprContainsUnsafeLogicalCallLike (expr : Expr) : Bool :=
     Expr.bitAnd a b | Expr.bitOr a b | Expr.bitXor a b | Expr.shl a b | Expr.shr a b
   | Expr.sar a b | Expr.signextend a b |
     Expr.eq a b | Expr.ge a b | Expr.gt a b | Expr.sgt a b | Expr.lt a b | Expr.slt a b | Expr.le a b |
-    Expr.wMulDown a b =>
+    Expr.wMulDown a b | Expr.ceilDiv a b =>
       exprContainsUnsafeLogicalCallLike a || exprContainsUnsafeLogicalCallLike b
   | Expr.mulDivDown a b c =>
       exprContainsUnsafeLogicalCallLike a || exprContainsUnsafeLogicalCallLike b || exprContainsUnsafeLogicalCallLike c
